Add IP and start bytes->values lemmas

proofs/FEC/Endian.v
@@ -1,6 +1,7 @@
 Require Import VST.floyd.functional_base.
 Require Import compcert.common.Memdata. (*for [int_of_bytes] and [bytes_of_int]*)
 Require Import ByteFacts.
+Set Bullet Behavior "Strict Subproofs".
 
 (** 4 and 16-bit integers *)
 
@@ -26,13 +27,53 @@ Notation short := Short.int.
 
 (*Combine nibbles into a byte (n1, followed by n2, in bits)*)
 Definition nibbles_to_Z (n1 n2: nibble) : Z :=
-  (Nibble.unsigned n1) + 16 * (Nibble.unsigned n2).
+  Z.lor (Nibble.unsigned n1) (Z.shiftl (Nibble.unsigned n2) 4).
+
+Lemma Z_testbit_false_le: forall (x y : Z),
+  0 <= x -> 0 < y ->
+  (forall i, i >= y -> Z.testbit x i = false) ->
+  x < 2 ^ y.
+Proof.
+  intros x y Hx Hy Hbits. assert (x > 0 \/ x <= 0) as [Hpos | Hneg] by lia. 2: lia.
+  apply Z.log2_lt_pow2; try lia.
+  rewrite <- (Z.log2_pow2 y) by lia. apply (testbit_lt (m:=y)); try lia.
+  replace 2 with (2^1) at 1 by reflexivity. apply Z.pow_le_mono_r; lia.
+  intros n Hn. apply Hbits. lia. apply Z.pow2_bits_true. lia.
+Qed.
+
+(*Need generic lemma about Z.lor bound*)
+Lemma Z_lor_bound: forall (z1 z2 i: Z),
+  0 < i ->
+  0 <= z1 < 2 ^ i ->
+  0 <= z2 < 2 ^ i ->
+  0 <= Z.lor z1 z2 < 2 ^ i.
+Proof.
+  intros z1 z2 i Hi Hz1 Hz2.
+  split.
+  - apply Z.lor_nonneg. split; lia.
+  - assert (z1 = 0 \/ 0 < z1) as [Hz1' | Hz1'] by lia.
+    + subst. rewrite Z.lor_0_l. lia.
+    + assert (z2 = 0 \/ 0 < z2) as [Hz2' |Hz2'] by lia.
+      * subst. rewrite Z.lor_0_r. lia.
+      * apply Z_testbit_false_le; try lia. apply Z.lor_nonneg. split; lia.
+        intros j Hj. rewrite Z.lor_spec. 
+        rewrite !Z.bits_above_log2; try lia; apply Z.log2_lt_pow2; try lia; eapply Z.lt_le_trans.
+        apply (proj2 Hz2). apply Z.pow_le_mono_r; lia. apply (proj2 Hz1). apply Z.pow_le_mono_r; lia.
+Qed.
+
 Lemma nibbles_to_Z_bound: forall n1 n2,
   -1 < (nibbles_to_Z n1 n2) < Byte.modulus.
 Proof.
-  intros. unfold nibbles_to_Z. pose proof (Nibble.unsigned_range n1).
-  pose proof (Nibble.unsigned_range n2).
-  assert (Nibble.modulus = 16) by reflexivity. rep_lia.
+  intros. unfold nibbles_to_Z.
+  assert (0 <= Z.lor (Nibble.unsigned n1) (Z.shiftl (Nibble.unsigned n2) 4) < 2 ^ 8). {
+    assert (Nibble.modulus = 16) by reflexivity.
+    apply Z_lor_bound. lia. pose proof (Nibble.unsigned_range n1).
+    assert (Nibble.modulus = 16) by reflexivity. lia.
+    pose proof (Nibble.unsigned_range n2).
+    split. apply Z.shiftl_nonneg. lia.
+    rewrite Z.shiftl_mul_pow2 by lia. replace (2^8) with (2^4 * 2^4) by reflexivity.
+    apply Zmult_lt_compat_r; lia. }
+  replace (Byte.modulus) with 256 by reflexivity. lia.
 Qed.
 
 (*Utility lemmas: should move or something*)
@@ -212,7 +253,7 @@ End Convert.
 (* This provides a shorthand to take machine-length types and represent as a list of bytes
   TODO; eventually this will be used to write short data_at representations*)
 
-Import ListNotations.
+Export ListNotations.
 
 Inductive MemBytes : Type :=
   | NibbleMem (n1: nibble) (n2: nibble)
@@ -230,3 +271,61 @@ Definition MemBytes_to_bytes (m: MemBytes) : list byte :=
 
 Definition MemBytes_to_byte_list (l: list MemBytes) : list byte :=
   List.flat_map MemBytes_to_bytes l.
+
+(** Convert bytes to primitive types *)
+
+(* Gives: lower 4 bits, higher 4 bits*)
+Definition byte_to_nibbles (b: byte) : nibble * nibble :=
+  (Nibble.repr (Z.land 15 (Byte.unsigned b)), Nibble.repr (Z.shiftr (Byte.unsigned b) 4)).
+
+Lemma byte_simpl: forall (i: Z) (Hi: -1 < i < Byte.modulus),
+  Byte.intval {| Byte.intval := i; Byte.intrange := Hi |} = i.
+Proof.
+  intros. reflexivity.
+Qed.
+
+(*This is much harder to prove than it seems
+  TODO: is there an easier way?*)
+Lemma byte_to_nibbles_inv: forall b,
+  let (n1, n2) := byte_to_nibbles b in
+  nibbles_to_byte n1 n2 = b.
+Proof.
+  intros b. unfold byte_to_nibbles. unfold nibbles_to_byte. apply byte_unsigned_inj.
+  rewrite byte_simpl. unfold nibbles_to_Z.
+  rewrite !Nibble.unsigned_repr.
+  - apply Z.bits_inj_iff. unfold Z.eqf. intros n.
+    assert (H15n: (Z.testbit 15 n = true) <-> 0 <= n < 4). {
+      split; intros.
+      - assert (0 <= n < 4 \/ n < 0 \/ n >= 4) as [Hin |[ Hlo | Hhi]] by lia.
+        + lia.
+        + rewrite Z.testbit_neg_r in H by lia. inversion H.
+        + rewrite Z.bits_above_log2 in H; try lia. 
+          replace (Z.log2 15) with 3 by reflexivity. lia.
+      - assert (n= 0 \/ n = 1 \/ n = 2 \/ n = 3) as [H1 | [H2 | [H3 | H4]]] by lia; subst; reflexivity. } 
+    rewrite Z.lor_spec,Z.land_spec.
+    assert (n < 0 \/ 0 <= n < 4 \/ 4 <= n) as [Hout |[Hfst | Hsnd]] by lia.
+    + assert (Z.testbit 15 n = false). { destruct (Z.testbit 15 n) eqn : Ht; auto. lia. }
+      rewrite H,andb_false_l,orb_false_l.
+      rewrite !Z.testbit_neg_r; lia.
+    + rewrite Z.shiftl_spec by lia.
+      replace (Z.testbit 15 n) with true. 2 : { symmetry; apply H15n; lia. }
+      simpl.
+      assert (Z.testbit (Z.shiftr (Byte.unsigned b) 4) (n - 4) = false). {
+        rewrite Z.testbit_neg_r; auto. lia. } rewrite H. rewrite orb_false_r. reflexivity.
+    + assert (Z.testbit 15 n = false). { destruct (Z.testbit 15 n) eqn : Ht; auto. lia. }
+      rewrite H,andb_false_l,orb_false_l.
+      rewrite Z.shiftl_spec by lia. rewrite Z.shiftr_spec by lia.
+      f_equal. lia.
+  - split.
+    + apply Z.shiftr_nonneg. pose proof (Byte.unsigned_range b); lia.
+    + rewrite Z.shiftr_div_pow2 by lia. replace (Nibble.max_unsigned) with 15 by reflexivity.
+      pose proof (Byte.unsigned_range b). replace (Byte.modulus) with 256 in H by reflexivity.
+      eapply Z.le_trans. apply Z.div_le_mono. lia. assert (Byte.unsigned b <= 255) by lia. apply H0.
+      replace (2^4) with 16 by reflexivity. 
+      replace (255 /16) with 15 by reflexivity. lia.
+  - split. 
+    + rewrite Z.land_nonneg. left. lia.
+    + replace (Nibble.max_unsigned) with 15 by reflexivity. apply Zbits.Ztestbit_le. lia.
+      intros i Hi. rewrite Z.land_spec, andb_true_iff. intros [Hi1 Hi2].
+      apply Hi1.
+Qed.
